refactor: make AIG parametric over atom type

LeanSAT/AIG/Basic.lean
@@ -22,7 +22,7 @@ theorem Array.get_push_size (as : Array α) (a : α) : (as.push a)[as.size] = a 
 /--
 A circuit node declaration. These are not recursive but instead contain indices into an `AIG`.
 -/
-inductive Decl where
+inductive Decl (α : Type) where
   /--
   A node with a constant output value.
   -/
@@ -30,7 +30,7 @@ inductive Decl where
   /--
   An input node to the circuit.
   -/
-  | atom (idx : Nat)
+  | atom (idx : α)
   /--
   An AIG gate with configurable input nodes and polarity. `l` and `r` are the
   input node indices while `linv` and `rinv` say whether there is an inverter on
@@ -39,12 +39,14 @@ inductive Decl where
   | gate (l r : Nat) (linv rinv : Bool)
   deriving BEq, Hashable, Repr, DecidableEq
 
+variable {α : Type} [BEq α] [Hashable α] [DecidableEq α]
+
 /--
 A `Cache` is valid with respect to a list of declarations iff:
 Whenever `cache.find? decl` returns an index into `xs : Array Decl`, `xs[index] = decl`.
 This predicate limits a `HashMap Decl Nat` to this behavior.
 -/
-inductive Cache.WF : Array Decl → HashMap Decl Nat → Prop where
+inductive Cache.WF : Array (Decl α) → HashMap (Decl α) Nat → Prop where
   /--
   An empty `Cache` is valid for any `Array Decl` as it never has a hit.
   -/
@@ -63,23 +65,24 @@ inductive Cache.WF : Array Decl → HashMap Decl Nat → Prop where
 /--
 A cache that is valid with respect to some `Array Decl`.
 -/
-def Cache (decls : Array Decl) := { map : HashMap Decl Nat // Cache.WF decls map }
+def Cache (α : Type) [BEq α] [Hashable α] (decls : Array (Decl α)) :=
+  { map : HashMap (Decl α) Nat // Cache.WF decls map }
 
 /--
 Create an empty `Cache`, valid with respect to any `Array Decl`.
 -/
 @[irreducible]
-def Cache.empty (decls : Array Decl) : Cache decl := ⟨HashMap.empty, WF.empty⟩
+def Cache.empty (decls : Array (Decl α)) : Cache α decl := ⟨HashMap.empty, WF.empty⟩
 
 @[inherit_doc Cache.WF.push_id, irreducible]
-def Cache.noUpdate (cache : Cache decls) : Cache (decls.push decl) :=
+def Cache.noUpdate (cache : Cache α decls) : Cache α (decls.push decl) :=
   ⟨cache.val, Cache.WF.push_id cache.property⟩
 
 @[inherit_doc Cache.WF.push_cache, irreducible]
-def Cache.insert (cache : Cache decls) (decl : Decl) : Cache (decls.push decl) :=
+def Cache.insert (cache : Cache α decls) (decl : Decl α) : Cache α (decls.push decl) :=
   ⟨cache.val.insert decl decls.size, Cache.WF.push_cache cache.property⟩
 
-structure CacheHit (decls : Array Decl) (decl : Decl) where
+structure CacheHit (decls : Array (Decl α)) (decl : Decl α) where
   idx : Nat
   hbound : idx < decls.size
   hvalid : decls[idx]'hbound = decl
@@ -90,7 +93,7 @@ Lookup a `decl` in a `cache`.
 If this returns `some i`, `Cache.find?_poperty` can be used to demonstrate: `decls[i] = decl`.
 -/
 @[irreducible]
-def Cache.find? (cache : Cache decls) (decl : Decl) : Option (CacheHit decls decl) :=
+def Cache.find? (cache : Cache α decls) (decl : Decl α) : Option (CacheHit decls decl) :=
   match cache.val.find? decl with
   | some hit =>
     /-
@@ -114,49 +117,49 @@ def Cache.find? (cache : Cache decls) (decl : Decl) : Option (CacheHit decls dec
 /--
 An `Array Decl` is a Direct Acyclic Graph (DAG) if this holds.
 -/
-def IsDag (decls : Array Decl) : Prop := ∀ i lhs rhs linv rinv (h : i < decls.size), decls[i] = .gate lhs rhs linv rinv → lhs < i ∧ rhs < i
+def IsDag (α : Type) (decls : Array (Decl α)) : Prop := ∀ i lhs rhs linv rinv (h : i < decls.size), decls[i] = .gate lhs rhs linv rinv → lhs < i ∧ rhs < i
 
 /--
 The empty array is a DAG.
 -/
-theorem IsDag.empty : IsDag #[] := by
+theorem IsDag.empty : IsDag α #[] := by
   intro i lhs rhs linv rinv h
   simp only [Array.size_toArray, List.length_nil] at h
   omega
 
 /--
-An And Inverter Graph (AIG) together with a cache for subterm sharing.
+An And Inverter Graph (AIG α) together with a cache for subterm sharing.
 -/
-structure AIG where
+structure AIG (α : Type) [BEq α] [Hashable α] where
   /--
   The circuit itself as an `Array Decl` whose members have indices into said array.
   -/
-  decls : Array Decl
+  decls : Array (Decl α)
   /--
   The `Decl` cache, valid with respect to `decls`.
   -/
-  cache : Cache decls
+  cache : Cache α decls
   /--
   In order to be a valid AIG, `decls` must form a DAG.
   -/
-  inv : IsDag decls
+  inv : IsDag α decls
 
 namespace AIG
 
 /--
 An `AIG` with an empty AIG and cache.
 -/
-def empty : AIG := { decls := #[], cache := Cache.empty #[], inv := IsDag.empty }
+def empty : AIG α := { decls := #[], cache := Cache.empty #[], inv := IsDag.empty }
 
 /--
 An entrypoint into an `AIG`. This can be used to evaluate a circuit, starting at a certain node,
 with `AIG.denote` or to construct bigger circuits
 -/
-structure Entrypoint where
+structure Entrypoint (α : Type) [BEq α] [Hashable α] where
   /--
   The AIG that we are in.
   -/
-  aig : AIG
+  aig : AIG α
   /--
   The AIG node at which to begin evaluation.
   -/
@@ -169,10 +172,10 @@ structure Entrypoint where
 /--
 Evaluate an `AIG.Entrypoint` using some assignment for atoms.
 -/
-def denote (entry : Entrypoint) (assign : Nat → Bool) : Bool :=
+def denote (entry : Entrypoint α) (assign : α → Bool) : Bool :=
   go entry.start entry.aig.decls assign entry.inv entry.aig.inv
 where
-  go (x : Nat) (decls : Array Decl) (assign : Nat → Bool) (h1 : x < decls.size) (h2 : IsDag decls) :=
+  go (x : Nat) (decls : Array (Decl α)) (assign : α → Bool) (h1 : x < decls.size) (h2 : IsDag α decls) :=
     match h3 : decls[x] with
     | .const b => b
     | .atom v => assign v
@@ -195,15 +198,15 @@ def unexpandDenote : Lean.PrettyPrinter.Unexpander
   | `($(_) $entry $assign) => `(⟦$entry, $assign⟧)
   | _ => throw ()
 
-def unsatAt (aig : AIG) (start : Nat) (h : start < aig.decls.size) : Prop := ∀ assign, ⟦aig, ⟨start, h⟩, assign⟧ = false
-def Entrypoint.unsat (entry : Entrypoint) : Prop := entry.aig.unsatAt entry.start entry.inv
+def unsatAt (aig : AIG α) (start : Nat) (h : start < aig.decls.size) : Prop := ∀ assign, ⟦aig, ⟨start, h⟩, assign⟧ = false
+def Entrypoint.unsat (entry : Entrypoint α) : Prop := entry.aig.unsatAt entry.start entry.inv
 
 /--
 Build an AIG gate in `aig`. Note that his version is only meant for proving,
 for production purposes use `AIG.mkGateCached` and equality theorems to this one.
 -/
-def mkGate (lhs rhs : Nat) (linv rinv : Bool) (aig : AIG) (hl : lhs < aig.decls.size)
-    (hr : rhs < aig.decls.size) : Entrypoint :=
+def mkGate (lhs rhs : Nat) (linv rinv : Bool) (aig : AIG α) (hl : lhs < aig.decls.size)
+    (hr : rhs < aig.decls.size) : Entrypoint α :=
   let g := aig.decls.size
   let decls := aig.decls.push (.gate lhs rhs linv rinv)
   let cache := aig.cache.noUpdate
@@ -219,7 +222,7 @@ def mkGate (lhs rhs : Nat) (linv rinv : Bool) (aig : AIG) (hl : lhs < aig.decls.
 Add a new input node to the AIG in `aig`. Note that his version is only meant for proving,
 for production purposes use `AIG.mkAtomCached` and equality theorems to this one.
 -/
-def mkAtom (n : Nat) (aig : AIG) : Entrypoint :=
+def mkAtom (n : α) (aig : AIG α) : Entrypoint α :=
   let g := aig.decls.size
   let decls := aig.decls.push (.atom n)
   let cache := aig.cache.noUpdate
@@ -236,7 +239,7 @@ def mkAtom (n : Nat) (aig : AIG) : Entrypoint :=
 Build an constant node in `aig`. Note that his version is only meant for proving,
 for production purposes use `AIG.mkConstCached` and equality theorems to this one.
 -/
-def mkConst (val : Bool) (aig : AIG) : Entrypoint :=
+def mkConst (val : Bool) (aig : AIG α) : Entrypoint α :=
   let g := aig.decls.size
   let decls := aig.decls.push (.const val)
   let cache := aig.cache.noUpdate
