LeanSAT/AIG/CachedLemmas.lean
@@ -13,10 +13,12 @@ in different scenarios. In particular reductions to the semantics of the non cac
 
 namespace AIG
 
+variable {α : Type} [BEq α] [Hashable α] [DecidableEq α]
+
 /--
 If we find a cached gate declaration in the AIG, denoting it is equivalent to denoting `AIG.mkGate`.
 -/
-theorem denote_mkGate_cached {aig : AIG} {hl} {hr} {hit}
+theorem denote_mkGate_cached {aig : AIG α} {hl} {hr} {hit}
     (h : aig.cache.find? (.gate lhs rhs lpol rpol) = some hit) :
     ⟦⟨aig, hit.idx, hit.hbound⟩, assign⟧
       =
@@ -31,7 +33,7 @@ theorem denote_mkGate_cached {aig : AIG} {hl} {hr} {hit}
 /--
 `AIG.mkGateCached` never shrinks the underlying AIG.
 -/
-theorem mkGateCached_le_size (aig : AIG) (lhs rhs : Nat) (linv rinv : Bool) hl hr
+theorem mkGateCached_le_size (aig : AIG α) (lhs rhs : Nat) (linv rinv : Bool) hl hr
     : aig.decls.size ≤ (aig.mkGateCached lhs rhs linv rinv hl hr).aig.decls.size := by
   dsimp [mkGateCached]
   split
@@ -41,7 +43,7 @@ theorem mkGateCached_le_size (aig : AIG) (lhs rhs : Nat) (linv rinv : Bool) hl h
 /--
 We can show that something is < the output AIG of `mkGateCached` by showing that it is < the input AIG.
 -/
-theorem lt_mkGateCached_size_of_lt_aig_size (aig : AIG) (lhs rhs : Nat) (linv rinv : Bool) (hl) (hr) (h : x < aig.decls.size)
+theorem lt_mkGateCached_size_of_lt_aig_size (aig : AIG α) (lhs rhs : Nat) (linv rinv : Bool) (hl) (hr) (h : x < aig.decls.size)
     : x < (aig.mkGateCached lhs rhs linv rinv hl hr).aig.decls.size := by
   have := mkGateCached_le_size aig lhs rhs linv rinv hl hr
   omega
@@ -49,7 +51,7 @@ theorem lt_mkGateCached_size_of_lt_aig_size (aig : AIG) (lhs rhs : Nat) (linv ri
 /--
 We can show that something is ≤ the output AIG of `mkGateCached` by showing that it is ≤ the input AIG.
 -/
-theorem le_mkGateCached_size_of_le_aig_size (aig : AIG) (lhs rhs : Nat) (linv rinv : Bool) (hl) (hr) (h : x ≤ aig.decls.size)
+theorem le_mkGateCached_size_of_le_aig_size (aig : AIG α) (lhs rhs : Nat) (linv rinv : Bool) (hl) (hr) (h : x ≤ aig.decls.size)
     : x ≤ (aig.mkGateCached lhs rhs linv rinv hl hr).aig.decls.size := by
   have := mkGateCached_le_size aig lhs rhs linv rinv hl hr
   omega
@@ -58,7 +60,7 @@ theorem le_mkGateCached_size_of_le_aig_size (aig : AIG) (lhs rhs : Nat) (linv ri
 Reusing an `AIG.Entrypoint` to build an additional gate will never invalidate the entry node of
 the original entrypoint.
 -/
-theorem lt_mkGateCached_size (entry : Entrypoint) (lhs rhs : Nat) (linv rinv : Bool) hl hr
+theorem lt_mkGateCached_size (entry : Entrypoint α) (lhs rhs : Nat) (linv rinv : Bool) hl hr
     : entry.start < (entry.aig.mkGateCached lhs rhs linv rinv hl hr).aig.decls.size := by
   apply lt_mkGateCached_size_of_lt_aig_size
   exact entry.inv
@@ -66,7 +68,7 @@ theorem lt_mkGateCached_size (entry : Entrypoint) (lhs rhs : Nat) (linv rinv : B
 /--
 `mkGateCached` does not modify the input AIG upon a cache hit.
 -/
-theorem mkGateCached_hit_aig (aig : AIG) {hit} (hcache : aig.cache.find? (.gate lhs rhs linv rinv) = some hit) (hl) (hr) :
+theorem mkGateCached_hit_aig (aig : AIG α) {hit} (hcache : aig.cache.find? (.gate lhs rhs linv rinv) = some hit) (hl) (hr) :
     (aig.mkGateCached lhs rhs linv rinv hl hr).aig = aig := by
   simp only [mkGateCached]
   split <;> simp_all
@@ -74,7 +76,7 @@ theorem mkGateCached_hit_aig (aig : AIG) {hit} (hcache : aig.cache.find? (.gate 
 /--
 `mkGateCached` pushes to the input AIG upon a cache miss.
 -/
-theorem mkGateCached_miss_aig (aig : AIG) (hcache : aig.cache.find? (.gate lhs rhs linv rinv) = none) (hl) (hr) :
+theorem mkGateCached_miss_aig (aig : AIG α) (hcache : aig.cache.find? (.gate lhs rhs linv rinv) = none) (hl) (hr) :
     (aig.mkGateCached lhs rhs linv rinv hl hr).aig.decls = aig.decls.push (.gate lhs rhs linv rinv) := by
   simp only [mkGateCached]
   split <;> simp_all
@@ -82,7 +84,7 @@ theorem mkGateCached_miss_aig (aig : AIG) (hcache : aig.cache.find? (.gate lhs r
 /--
 The AIG produced by `AIG.mkGateCached` agrees with the input AIG on all indices that are valid for both.
 -/
-theorem mkGateCached_decl_eq idx (aig : AIG) (lhs rhs : Nat) (linv rinv : Bool)
+theorem mkGateCached_decl_eq idx (aig : AIG α) (lhs rhs : Nat) (linv rinv : Bool)
     {h : idx < aig.decls.size} {hl} {hr} {hbound} :
     (aig.mkGateCached lhs rhs linv rinv hl hr).aig.decls[idx]'hbound = aig.decls[idx] := by
   match hcache:aig.cache.find? (.gate lhs rhs linv rinv) with
@@ -99,7 +101,7 @@ theorem mkGateCached_decl_eq idx (aig : AIG) (lhs rhs : Nat) (linv rinv : Bool)
 /--
 The input AIG to an `AIG.mkGateCached` is a prefix to the output AIG.
 -/
-theorem mkGateCached_IsPrefix_aig {aig : AIG} {hl} {hr} :
+theorem mkGateCached_IsPrefix_aig {aig : AIG α} {hl} {hr} :
     IsPrefix aig.decls (aig.mkGateCached lhs rhs lpol rpol hl hr).aig.decls := by
   apply IsPrefix.of
   . intro idx h
@@ -107,14 +109,14 @@ theorem mkGateCached_IsPrefix_aig {aig : AIG} {hl} {hr} :
   . apply mkGateCached_le_size
 
 @[simp]
-theorem denote_mkGateCached_entry (entry : Entrypoint) {hlbound} {hrbound} {h} :
+theorem denote_mkGateCached_entry (entry : Entrypoint α) {hlbound} {hrbound} {h} :
     ⟦(entry.aig.mkGateCached lhs rhs lpol rpol hlbound hrbound).aig, ⟨entry.start, h⟩, assign ⟧
       =
     ⟦entry, assign⟧ :=  by
   apply denote.eq_of_aig_eq
   apply mkGateCached_IsPrefix_aig
 
-theorem denote_mkGateCached_mem_prefix {aig : AIG} {hlbound} {hrbound} (h) :
+theorem denote_mkGateCached_mem_prefix {aig : AIG α} {hlbound} {hrbound} (h) :
     ⟦(aig.mkGateCached lhs rhs lpol rpol hlbound hrbound).aig, ⟨start, (by apply lt_mkGateCached_size_of_lt_aig_size; assumption)⟩, assign ⟧
       =
     ⟦aig, ⟨start, h⟩, assign⟧ :=  by
@@ -124,7 +126,7 @@ theorem denote_mkGateCached_mem_prefix {aig : AIG} {hlbound} {hrbound} (h) :
 The central equality theorem between `mkGateCached` and `mkGate`.
 -/
 @[simp]
-theorem mkGateCached_eval_eq_mkGate_eval {aig : AIG} {hl} {hr} :
+theorem mkGateCached_eval_eq_mkGate_eval {aig : AIG α} {hl} {hr} :
     ⟦aig.mkGateCached lhs rhs linv rinv hl hr, assign⟧ = ⟦aig.mkGate lhs rhs linv rinv hl hr, assign⟧ := by
   simp only [mkGateCached]
   split
@@ -135,7 +137,7 @@ theorem mkGateCached_eval_eq_mkGate_eval {aig : AIG} {hl} {hr} :
 /--
 If we find a cached atom declaration in the AIG, denoting it is equivalent to denoting `AIG.mkAtom`.
 -/
-theorem denote_mkAtom_cached {aig : AIG} {hit} (h : aig.cache.find? (.atom v) = some hit) :
+theorem denote_mkAtom_cached {aig : AIG α} {hit} (h : aig.cache.find? (.atom v) = some hit) :
     ⟦aig, ⟨hit.idx, hit.hbound⟩, assign⟧ = ⟦aig.mkAtom v, assign⟧ := by
   have := hit.hvalid
   simp only [denote_mkAtom]
@@ -145,7 +147,7 @@ theorem denote_mkAtom_cached {aig : AIG} {hit} (h : aig.cache.find? (.atom v) = 
 /--
 `mkAtomCached` does not modify the input AIG upon a cache hit.
 -/
-theorem mkAtomCached_hit_aig (aig : AIG) {hit} (hcache : aig.cache.find? (.atom var) = some hit) :
+theorem mkAtomCached_hit_aig (aig : AIG α) {hit} (hcache : aig.cache.find? (.atom var) = some hit) :
     (aig.mkAtomCached var).aig = aig := by
   simp only [mkAtomCached]
   split <;> simp_all
@@ -153,7 +155,7 @@ theorem mkAtomCached_hit_aig (aig : AIG) {hit} (hcache : aig.cache.find? (.atom 
 /--
 `mkAtomCached` pushes to the input AIG upon a cache miss.
 -/
-theorem mkAtomCached_miss_aig (aig : AIG) (hcache : aig.cache.find? (.atom var) = none) :
+theorem mkAtomCached_miss_aig (aig : AIG α) (hcache : aig.cache.find? (.atom var) = none) :
     (aig.mkAtomCached var).aig.decls = aig.decls.push (.atom var) := by
   simp only [mkAtomCached]
   split <;> simp_all
@@ -161,7 +163,7 @@ theorem mkAtomCached_miss_aig (aig : AIG) (hcache : aig.cache.find? (.atom var) 
 /--
 The AIG produced by `AIG.mkAtomCached` agrees with the input AIG on all indices that are valid for both.
 -/
-theorem mkAtomCached_decl_eq (aig : AIG) (var : Nat) (idx : Nat) {h : idx < aig.decls.size} {hbound} :
+theorem mkAtomCached_decl_eq (aig : AIG α) (var : α) (idx : Nat) {h : idx < aig.decls.size} {hbound} :
     (aig.mkAtomCached var).aig.decls[idx]'hbound = aig.decls[idx] := by
   match hcache:aig.cache.find? (.atom var) with
   | some gate =>
@@ -177,7 +179,7 @@ theorem mkAtomCached_decl_eq (aig : AIG) (var : Nat) (idx : Nat) {h : idx < aig.
 /--
 `AIG.mkAtomCached` never shrinks the underlying AIG.
 -/
-theorem mkAtomCached_le_size (aig : AIG) (var : Nat)
+theorem mkAtomCached_le_size (aig : AIG α) (var : α)
     : aig.decls.size ≤ (aig.mkAtomCached var).aig.decls.size := by
   dsimp [mkAtomCached]
   split
@@ -188,7 +190,7 @@ theorem mkAtomCached_le_size (aig : AIG) (var : Nat)
 The central equality theorem between `mkAtomCached` and `mkAtom`.
 -/
 @[simp]
-theorem mkAtomCached_eval_eq_mkAtom_eval {aig : AIG}
+theorem mkAtomCached_eval_eq_mkAtom_eval {aig : AIG α}
     : ⟦aig.mkAtomCached var, assign⟧ = ⟦aig.mkAtom var, assign⟧ := by
   simp only [mkAtomCached]
   split
@@ -199,7 +201,7 @@ theorem mkAtomCached_eval_eq_mkAtom_eval {aig : AIG}
 /--
 If we find a cached const declaration in the AIG, denoting it is equivalent to denoting `AIG.mkConst`.
 -/
-theorem denote_mkConst_cached {aig : AIG} {hit} (h : aig.cache.find? (.const b) = some hit) :
+theorem denote_mkConst_cached {aig : AIG α} {hit} (h : aig.cache.find? (.const b) = some hit) :
     ⟦aig, ⟨hit.idx, hit.hbound⟩, assign⟧ = ⟦aig.mkConst b, assign⟧ := by
   have := hit.hvalid
   simp only [denote_mkConst]
@@ -209,7 +211,7 @@ theorem denote_mkConst_cached {aig : AIG} {hit} (h : aig.cache.find? (.const b) 
 /--
 `mkConstCached` does not modify the input AIG upon a cache hit.
 -/
-theorem mkConstCached_hit_aig (aig : AIG) {hit} (hcache : aig.cache.find? (.const val) = some hit) :
+theorem mkConstCached_hit_aig (aig : AIG α) {hit} (hcache : aig.cache.find? (.const val) = some hit) :
     (aig.mkConstCached val).aig = aig := by
   simp only [mkConstCached]
   split <;> simp_all
@@ -217,7 +219,7 @@ theorem mkConstCached_hit_aig (aig : AIG) {hit} (hcache : aig.cache.find? (.cons
 /--
 `mkConstCached` pushes to the input AIG upon a cache miss.
 -/
-theorem mkConstCached_miss_aig (aig : AIG) (hcache : aig.cache.find? (.const val) = none) :
+theorem mkConstCached_miss_aig (aig : AIG α) (hcache : aig.cache.find? (.const val) = none) :
     (aig.mkConstCached val).aig.decls = aig.decls.push (.const val) := by
   simp only [mkConstCached]
   split <;> simp_all
@@ -225,7 +227,7 @@ theorem mkConstCached_miss_aig (aig : AIG) (hcache : aig.cache.find? (.const val
 /--
 The AIG produced by `AIG.mkConstCached` agrees with the input AIG on all indices that are valid for both.
 -/
-theorem mkConstCached_decl_eq (aig : AIG) (val : Bool) (idx : Nat) {h : idx < aig.decls.size} {hbound} :
+theorem mkConstCached_decl_eq (aig : AIG α) (val : Bool) (idx : Nat) {h : idx < aig.decls.size} {hbound} :
     (aig.mkConstCached val).aig.decls[idx]'hbound = aig.decls[idx] := by
   match hcache:aig.cache.find? (.const val) with
   | some gate =>
@@ -241,7 +243,7 @@ theorem mkConstCached_decl_eq (aig : AIG) (val : Bool) (idx : Nat) {h : idx < ai
 /--
 `AIG.mkConstCached` never shrinks the underlying AIG.
 -/
-theorem mkConstCached_le_size (aig : AIG) (val : Bool)
+theorem mkConstCached_le_size (aig : AIG α) (val : Bool)
     : aig.decls.size ≤ (aig.mkConstCached val).aig.decls.size := by
   dsimp [mkConstCached]
   split
@@ -251,7 +253,7 @@ theorem mkConstCached_le_size (aig : AIG) (val : Bool)
 /--
 We can show that something is < the output AIG of `mkConstCached` by showing that it is < the input AIG.
 -/
-theorem lt_mkConstCached_size_of_lt_aig_size (aig : AIG) (val : Bool) (h : x < aig.decls.size) :
+theorem lt_mkConstCached_size_of_lt_aig_size (aig : AIG α) (val : Bool) (h : x < aig.decls.size) :
     x < (aig.mkConstCached val).aig.decls.size := by
   have := mkConstCached_le_size aig val
   omega
@@ -259,7 +261,7 @@ theorem lt_mkConstCached_size_of_lt_aig_size (aig : AIG) (val : Bool) (h : x < a
 /--
 We can show that something is ≤ the output AIG of `mkConstCached` by showing that it is ≤ the input AIG.
 -/
-theorem le_mkConstCached_size_of_le_aig_size (aig : AIG) (val : Bool) (h : x ≤ aig.decls.size) :
+theorem le_mkConstCached_size_of_le_aig_size (aig : AIG α) (val : Bool) (h : x ≤ aig.decls.size) :
     x ≤ (aig.mkConstCached val).aig.decls.size := by
   have := mkConstCached_le_size aig val
   omega
@@ -268,27 +270,27 @@ theorem le_mkConstCached_size_of_le_aig_size (aig : AIG) (val : Bool) (h : x ≤
 Reusing an `AIG.Entrypoint` to build an additional constant will never invalidate the entry node of
 the original entrypoint.
 -/
-theorem lt_mkConstCached_size (entry : Entrypoint) : entry.start < (entry.aig.mkConstCached val).aig.decls.size := by
+theorem lt_mkConstCached_size (entry : Entrypoint α) : entry.start < (entry.aig.mkConstCached val).aig.decls.size := by
   have h1 := entry.inv
   have h2 : entry.aig.decls.size ≤ (entry.aig.mkConstCached val).aig.decls.size :=
     AIG.mkConstCached_le_size _ _
   omega
 
-theorem mkConstCached_IsPrefix_aig : IsPrefix aig.decls (mkConstCached val aig).aig.decls := by
+theorem mkConstCached_IsPrefix_aig {aig : AIG α} : IsPrefix aig.decls (mkConstCached val aig).aig.decls := by
   apply IsPrefix.of
   . intro idx h
     apply mkConstCached_decl_eq
   . apply mkConstCached_le_size
 
 @[simp]
-theorem denote_mkConstCached_entry (entry : Entrypoint) {h} :
+theorem denote_mkConstCached_entry (entry : Entrypoint α) {h} :
     ⟦(entry.aig.mkConstCached val).aig, ⟨entry.start, h⟩, assign⟧
       =
     ⟦entry, assign⟧ := by
   apply denote.eq_of_aig_eq
   apply mkConstCached_IsPrefix_aig
 
-theorem denote_mkConstCached_mem_prefix {aig : AIG} (h) :
+theorem denote_mkConstCached_mem_prefix {aig : AIG α} (h) :
     ⟦(aig.mkConstCached val).aig, ⟨start, by apply lt_mkConstCached_size_of_lt_aig_size; assumption⟩, assign⟧
       =
     ⟦aig, ⟨start, h⟩, assign⟧ := by
@@ -298,7 +300,7 @@ theorem denote_mkConstCached_mem_prefix {aig : AIG} (h) :
 The central equality theorem between `mkConstCached` and `mkConst`.
 -/
 @[simp]
-theorem mkConstCached_eval_eq_mkConst_eval {aig : AIG}
+theorem mkConstCached_eval_eq_mkConst_eval {aig : AIG α}
     : ⟦aig.mkConstCached val, assign⟧ = ⟦aig.mkConst val, assign⟧ := by
   simp only [mkConstCached]
   split
